WIP/exploration toward non-expansive substitution

theories/DMin/synNMOfeOpenSemTypes.v
@@ -12,6 +12,8 @@ From iris.proofmode Require Export tactics.
 Import uPred.
 
 From DN Require Import autosubst_preds DMin.synNonMutual DMin.synNMOfe.
+Require Import Program.Equality.
+Unset Program Cases.
 
 Canonical Structure varC: ofeT := leibnizC var.
 Section openSemanticSyntax.
@@ -89,9 +91,97 @@ Section openSemanticSyntax.
     λ r preD, λne ρ, preD (lift_varfun (r >>> ρ)).
   Solve All Obligations with solve_proper_cbn.
 
+  Global Instance Rename_lpreD : Rename (laterC preD) :=
+    λ r '(Next preD), Next (rename r preD).
+  Global Instance Rename_iSyn {s}: Rename (iSyn s) := _.
+
+  Global Instance hsubst_lpreD `{!HSubst vl preD} : HSubst vl (laterC preD) :=
+    λ sb '(Next preD), Next (hsubst sb preD).
+  Global Instance proper_hslpreD ρ `{!HSubst vl preD}
+    `{proper_hspreD: ∀ ρ, NonExpansive (λ v: preD, hsubst ρ v)}:
+    NonExpansive (λ v: laterC preD, hsubst ρ v).
+  Proof.
+    move => n [x] [y] H /=. rewrite /hsubst_lpreD.
+    f_contractive. by eapply proper_hspreD.
+  Qed.
+
+  Global Instance subst_prevl `{!HSubst vl preD} : Subst iPreVl :=
+    λ sb v, iSyn_unfold (subst (λ x, (iSyn_fold (sb x))) (iSyn_fold v)).
+
   (* This will probably need some Iris fixpoint.
     And we need to lift subst to the category of OFEs. *)
-  Fail Global Program Instance HSubst_pred : HSubst vl preD :=
+  Program Definition hsubst_preD (rec: (var → vl) → preD → preD): (var → vl) → preD → preD :=
+    let hsubst_preD' : HSubst vl preD := rec in
+    λ sb preD, λne ρ, preD (lift_varfun (sb >>> iSyn_unfold >>> @subst _ subst_prevl ρ)).
+  Next Obligation. intros **???. f_equiv. rewrite /lift_varfun => ? /=. f_equiv. Admitted.
+
+  Program Definition syn_rename_ofe {s}
+    `{proper_hrpreD1: ∀ ρ, NonExpansive (λ v: preD, rename ρ v)}
+    `{proper_hrpreD2: NonExpansive2 (λ (ρ: varC -n> varC) (v: preD), rename ρ v)}:
+    (varC -n> varC) -n> iSyn s -n> iSyn s :=
+    λne ρ v, syn_rename ρ v.
+  Next Obligation.
+    intros **???. move: s x y H ρ.
+    induction x; intros; inversion H; simplify_eq; cbn; f_equiv;
+      try by [apply IHx| apply IHx1 | apply IHx2|].
+    - by inversion H2.
+    - by unshelve eapply (IHx _ _ (λne x, upren ρ x)).
+    - by apply later_map_ne.
+      (* move: α α2 {H} H3 => [α] [α2] H3 /=. rewrite /Rename_lpreD.
+      f_contractive.
+      by eapply proper_hrpreD2. *)
+  Qed.
+  Next Obligation.
+    intros ** x y H t; move: x y H.
+    induction t; cbn; intros; f_equiv;
+    try by [apply IHt| apply IHt1 | apply IHt2|]; eauto.
+    - unshelve eapply (IHt (λne z, upren x z) (λne z, upren y z)).
+      move => [|m] //=. f_equiv. apply H.
+    - move: α => [α] /=. rewrite /Rename_lpreD.
+      (* f_contractive. *)
+      f_equiv; by eapply proper_hrpreD2.
+  Qed.
+  Fail Next Obligation.
+  Program Definition syn_hsubst_ofe {s} {hspreD: HSubst vl preD}
+    `{proper_hrpreD1: ∀ ρ, NonExpansive (λ v: preD, rename ρ v)}
+    `{proper_hrpreD2: NonExpansive2 (λ (ρ: varC -n> varC) (v: preD), rename ρ v)}
+    `{proper_hspreD1: ∀ ρ, NonExpansive (λ v: preD, hsubst ρ v)}
+    `{proper_hspreD2: NonExpansive2 (λ (ρ: varC -n> vl) (v: preD), hsubst ρ v)}:
+    (varC -n> vl) -n> iSyn s -n> iSyn s :=
+    λne ρ v, syn_hsubst ρ v.
+  Next Obligation.
+    intros **???. move: s x y H ρ.
+    induction x; intros; inversion H; simplify_eq; cbn; f_equiv;
+      try by [apply IHx| apply IHx1 | apply IHx2|].
+    by unshelve eapply (IHx _ _ (λne x, up ρ x)).
+    by f_equiv.
+  Qed.
+  Next Obligation.
+    intros ** x y H t; move: x y H.
+    induction t; cbn; intros; f_equiv;
+    try by [apply IHt| apply IHt1 | apply IHt2|]; eauto.
+    - unshelve eapply (IHt (λne z, up x z) (λne z, up y z)).
+
+      (* Should have just proved that the existing function is non-expansive? *)
+      rewrite /up.
+      move => [|m] //=.
+      (* by f_equiv. *)
+      rewrite /rename.
+      replace Rename_syn with (λ (ρ: var -> var) (v: vl), (@syn_rename_ofe vls _ _ (λne x, ρ x) v));
+      by [f_equiv|].
+    - move: α => [α] /=. rewrite /hsubst_lpreD.
+      f_contractive.
+      eapply proper_hspreD2 => //. by apply dist_S.
+  Qed.
+
+
+  (* Global Instance proper_hspreD n ρ `{!HSubst vl preD} :
+    Proper (dist n ==> dist n) (λ v: preD, hsubst ρ v).
+  Proof. intros** x y H. *)
+
+  (* Global Program Instance syn_hsubst_ne s: NonExpansive2 (@syn_hsubst (laterC preD) _ _ s). *)
+  Fail Next Obligation.
+  Fail Global Program Instance HSubst_preD : HSubst vl preD :=
     λ sb preD, λne ρ, preD (lift_varfun (sb >>> iSyn_unfold >>> subst ρ)).
 
   (* XXX First I thought of lifting Autosubst functions to
